specialize directives extract to F*

src/3d/ocaml/lexer.mll
@@ -67,7 +67,8 @@ let () =
   H.add keywords "extern" EXTERN;
   H.add keywords "probe" PROBE;
   H.add keywords "pointer" POINTER;
-  H.add keywords "PURE" PURE
+  H.add keywords "PURE" PURE;
+  H.add keywords "specialize" SPECIALIZE
 
 let unsigned_int_of_string s = int_of_string (String.sub s 0 (String.length s - 2))
 
