src/3d/Binding.fsti
@@ -23,6 +23,10 @@ val mk_env (g:global_env) : ML env
 val global_env_of_env (e:env) : ML global_env
 
 val resolve_record_case_output_extern_type_name (_:env) (_:ident): ML ident
+val lookup_type_decl (_:env) (_:ident) : ML (decl & decl_attributes)
+val resolve_record_type (_:env) (_:ident) 
+: ML (res:(decl & decl_attributes) { Record? (fst res).d_decl.v })
+val params_of_decl (d:decl) : list generic_param & list param
 val lookup_expr_name (_:env) (_:ident) : ML typ
 val lookup_macro_definition (_:env) (_:ident) : ML (option expr)
 val has_reader (_:global_env) (_:ident) : ML bool
